@prefix dbo: <http://www.dbpedia.org/ontology/> .
@prefix dbr: <http://www.dbpedia.org/resource/> .
@prefix ex: <http://example.org/> .
@prefix foaf: <http://xmlns.com/foaf/0.1/> .
@prefix focu: <http://focu.io/schema#> .
@prefix rdf: <http://www.w3.org/1999/02/22-rdf-syntax-ns#> .
@prefix rdfs: <http://www.w3.org/2000/01/rdf-schema#> .
@prefix xsd: <http://www.w3.org/2001/XMLSchema#> .

focu:Student a rdfs:Class ;
    rdfs:label "Student"@en ;
    rdfs:comment "A person enrolled in one or more courses at a academic institution or other place of academic learning"@en ;
    rdfs:subClassOf foaf:Person .

ex:ACCO220 a <http://www.dbpedia.org/resource/Course_(education)> ;
    rdfs:label "Financial and Managerial Accounting" ;
    focu:catalog "220" ;
    focu:credits 3.0 ;
    focu:offeredAt ex:Concordia ;
    focu:provenance "Concordia Open Data" ;
    focu:subject "ACCO" ;
    rdfs:comment """This course provides an introduction to accounting principles underlying the preparation of financial reports with an emphasis on the relationship between accounting information and production decisions. It examines the relationship between costs, production volume, and profit, as well as the practical benefits of standard costs for planning and control purposes. The role of accounting information in various manufacturing decisions is also highlighted.

NOTE: This course would be useful to Engineering students.
NOTE: JMSB students may not take this course for credit.
NOTE: Students who have received credit for ACCO 230, 240 may not take this course for credit.""" ;
    rdfs:seeAlso "('Managerial Accounting', 'http://dbpedia.org/resource/Management_accounting')",
        "http://dbpedia.org/resource/Acre,_Israel" ;
    foaf:topic "ACCO",
        "Managerial Accounting",
        "accounting" .

ex:ACCO230 a <http://www.dbpedia.org/resource/Course_(education)> ;
    rdfs:label "Introduction to Financial Accounting" ;
    focu:catalog "230" ;
    focu:credits 3.0 ;
    focu:offeredAt ex:Concordia ;
    focu:provenance "Concordia Open Data" ;
    focu:subject "ACCO" ;
    rdfs:comment """This course provides an introduction to accounting concepts underlying financial statements of organizations. It focuses on the analysis, measurement, and reporting of business transactions to users of financial statements. It also examines the uses and limitations of accounting information for investment and credit decisions.

NOTE: JMSB students may not take this course for credit.
"NOTE: Students who receive a grade of ""C"" or better may be exempt from COMM 217."
NOTE: Students who have received credit for ACCO 220 may not take this course for credit.""" ;
    rdfs:seeAlso "('Accounting', 'http://dbpedia.org/resource/Accounting')",
        "http://dbpedia.org/resource/Acre,_Israel" ;
    foaf:topic "ACCO",
        "Accounting",
        "accounting",
        "financial statements" .

ex:ACCO240 a <http://www.dbpedia.org/resource/Course_(education)> ;
    rdfs:label "Introduction to Managerial Accounting" ;
    focu:catalog "240" ;
    focu:credits 3.0 ;
    focu:offeredAt ex:Concordia ;
    focu:provenance "Concordia Open Data" ;
    focu:subject "ACCO" ;
    rdfs:comment """This course examines the role of accounting information for decision making, and focuses on concepts and techniques used in planning operations, controlling activities, and evaluating managerial performance. New developments are addressed with a focus on contemporary business issues and real-world applicability of management accounting concepts and techniques.
Prerequisite: ACCO 230.
NOTE: JMSB students may not take this course for credit.
NOTE: Students who receive a passing grade may be exempt from COMM 305.
NOTE: Students who have received credit for ACCO 220 may not take this course for credit.""" ;
    rdfs:seeAlso "('Managerial Accounting', 'http://dbpedia.org/resource/Management_accounting')",
        "http://dbpedia.org/resource/Acre,_Israel" ;
    foaf:topic "ACCO",
        "Managerial Accounting",
        "accounting",
        "decision making" .

ex:ACCO310 a <http://www.dbpedia.org/resource/Course_(education)> ;
    rdfs:label "Financial Reporting I" ;
    focu:catalog "310" ;
    focu:credits 3.0 ;
    focu:offeredAt ex:Concordia ;
    focu:subject "ACCO" ;
    rdfs:comment """Intensive study is made of the theory and practice of external financial reporting by business organizations, focusing on concepts and procedures underlying the measurement of assets and the determination of income.
Prerequisite: COMM 305 previously or concurrently.""" ;
    foaf:topic "financial reporting" .

ex:ACCO320 a <http://www.dbpedia.org/resource/Course_(education)> ;
    rdfs:label "Financial Reporting II" ;
    focu:catalog "320" ;
    focu:credits 3.0 ;
    focu:offeredAt ex:Concordia ;
    focu:provenance "Concordia Open Data" ;
    focu:subject "ACCO" ;
    rdfs:comment """This course continues the intensive study of ACCO 310, with particular emphasis on accounting for liabilities, shareholders' equity, and other related topics such as earnings per share, pension accounting, and accounting for income taxes.
Prerequisite: ACCO 310.""" ;
    rdfs:seeAlso "('II', 'http://dbpedia.org/resource/World_War_II')",
        "http://dbpedia.org/resource/Acre,_Israel" ;
    foaf:topic "ACCO",
        "II",
        "accounting",
        "liabilities",
        "pension",
        "shareholders' equity" .

ex:ACCO330 a <http://www.dbpedia.org/resource/Course_(education)> ;
    rdfs:label "Cost and Management Accounting" ;
    focu:catalog "330" ;
    focu:credits 3.0 ;
    focu:offeredAt ex:Concordia ;
    focu:subject "ACCO" ;
    rdfs:comment """This course provides an examination of the techniques, systems, and procedures applicable to the managerial use of accounting information for planning, decision-making, and control. Topics include cost accumulation and allocation, product and process costing, flexible budgeting and variance analysis, evaluation of managerial performance, and transfer pricing.
Prerequisite: COMM 305.""" ;
    rdfs:seeAlso "('Management Accounting', 'http://dbpedia.org/resource/Management_accounting')" ;
    foaf:topic "Management Accounting",
        "accounting",
        "process costing",
        "transfer pricing",
        "variance analysis" .

ex:ACCO340 a <http://www.dbpedia.org/resource/Course_(education)> ;
    rdfs:label "Income Taxation in Canada" ;
    focu:catalog "340" ;
    focu:credits 3.0 ;
    focu:offeredAt ex:Concordia ;
    focu:subject "ACCO" ;
    rdfs:comment """This course provides core knowledge regarding the federal income tax structure and the Canadian goods and services tax system. It examines the taxation of employment, business, property income, capital gains and other sources of income for an individual.
Prerequisite: COMM 217.""" ;
    rdfs:seeAlso "('Canada', 'http://dbpedia.org/resource/Canada')" ;
    foaf:topic "Canada",
        "Canadian",
        "capital gains",
        "federal income tax",
        "goods",
        "property income",
        "tax" .

ex:ACCO350 a <http://www.dbpedia.org/resource/Course_(education)> ;
    rdfs:label "Accounting and Information Technology" ;
    focu:catalog "350" ;
    focu:credits 3.0 ;
    focu:offeredAt ex:Concordia ;
    focu:subject "ACCO" ;
    rdfs:comment """This course examines the role of computerized accounting information systems (AIS) in organizations. Students learn how to justify, design, and utilize AIS to provide pertinent information to managers for decision making. The course helps to identify appropriate usage of information technology in specific accounting contexts. Topics include e-business, computer fraud, information systems security and controls, systems analysis, and management of information technology.
Prerequisite: COMM 226 or 301, COMM 305""" ;
    rdfs:seeAlso "('Information Technology', 'http://dbpedia.org/resource/Information_technology')" ;
    foaf:topic "AIS",
        "Accounting",
        "Information Technology",
        "accounting",
        "computer",
        "decision making",
        "e-business",
        "fraud",
        "systems analysis" .

ex:ACCO355 a <http://www.dbpedia.org/resource/Course_(education)> ;
    rdfs:label "Analysis of Financial Statements" ;
    focu:catalog "355" ;
    focu:credits 3.0 ;
    focu:offeredAt ex:Concordia ;
    focu:subject "ACCO" ;
    rdfs:comment """This course explores the usefulness and limitations of financial statements for investment and credit decisions. It focuses on the interpretation of the information contained in financial statements which reflect the economic characteristics of the firm and its strategic business decisions. Instruments and techniques for financial statement analysis are discussed and applied to case studies and actual companies.
Prerequisite: COMM 305, 308.

NOTE: This course would be useful for students in Finance and Management.""" ;
    foaf:topic "financial statement analysis",
        "financial statements" .

ex:ACCO365 a <http://www.dbpedia.org/resource/Course_(education)> ;
    rdfs:label "U.S. Federal Taxation" ;
    focu:catalog "365" ;
    focu:credits 3.0 ;
    focu:offeredAt ex:Concordia ;
    focu:provenance "Concordia Open Data" ;
    focu:subject "ACCO" ;
    rdfs:comment """This course familiarizes the student with individual and corporate taxation in the U.S. The use of professional judgment in the application of tax planning recommendations is also addressed in this course.
Prerequisite: COMM 217 or ACCO 230.
NOTE: Students who have received credit for this topic under an ACCO 470 number may not take this course for credit.""" ;
    rdfs:seeAlso "('U.S.', 'http://dbpedia.org/resource/United_States')",
        "http://dbpedia.org/resource/Acre,_Israel" ;
    foaf:topic "ACCO",
        "U.S.",
        "corporate taxation",
        "tax planning" .

ex:ACCO400 a <http://www.dbpedia.org/resource/Course_(education)> ;
    rdfs:label "Accounting Theory" ;
    focu:catalog "400" ;
    focu:credits 3.0 ;
    focu:offeredAt ex:Concordia ;
    focu:provenance "Concordia Open Data" ;
    focu:subject "ACCO" ;
    rdfs:comment """This course examines the theoretical foundations of the contemporary approach to financial reporting, and the political and pragmatic considerations in the development of the conceptual framework underlying current accounting standards. Alternative theories of accounting are discussed and controversial areas are emphasized.
Prerequisite: ACCO 320.""" ;
    rdfs:seeAlso "('Accounting', 'http://dbpedia.org/resource/Accounting')",
        "http://dbpedia.org/resource/Acre,_Israel" ;
    foaf:topic "ACCO",
        "Accounting",
        "accounting",
        "conceptual framework",
        "financial reporting" .

ex:ACCO420 a <http://www.dbpedia.org/resource/Course_(education)> ;
    rdfs:label "Financial Reporting III" ;
    focu:catalog "420" ;
    focu:credits 3.0 ;
    focu:offeredAt ex:Concordia ;
    focu:provenance "Concordia Open Data" ;
    focu:subject "ACCO" ;
    rdfs:comment """This course examines the theory and practice of accounting for intercorporate investments, business combinations, consolidation of financial statements, and foreign currency transactions and operations.
Prerequisite: ACCO 320.""" ;
    rdfs:seeAlso "('III', 'http://dbpedia.org/resource/NCAA_Division_III')",
        "http://dbpedia.org/resource/Acre,_Israel" ;
    foaf:topic "ACCO",
        "accounting",
        "currency",
        "financial statements" .

ex:ACCO425 a <http://www.dbpedia.org/resource/Course_(education)> ;
    rdfs:label "FINANCIAL REPORTING IV" ;
    focu:catalog "425" ;
    focu:credits 3.0 ;
    focu:offeredAt ex:Concordia ;
    focu:subject "ACCO" ;
    rdfs:comment "Please see UGRD Calendar" ;
    rdfs:seeAlso "('IV', 'http://dbpedia.org/resource/Intravenous_therapy')" ;
    foaf:topic "IV" .

ex:ACCO430 a <http://www.dbpedia.org/resource/Course_(education)> ;
    rdfs:label "Advanced Management Accounting" ;
    focu:catalog "430" ;
    focu:credits 3.0 ;
    focu:offeredAt ex:Concordia ;
    focu:provenance "Concordia Open Data" ;
    focu:subject "ACCO" ;
    rdfs:comment """The course examines the integrative and interdisciplinary role of management accounting and its contribution to the complex management process. The course focuses on cases that deal with strategic issues in management accounting and management's need for both quantitative and qualitative information for planning, control, performance evaluation and decision making.
Prerequisite: ACCO 330.""" ;
    rdfs:seeAlso "('Management Accounting', 'http://dbpedia.org/resource/Management_accounting')",
        "http://dbpedia.org/resource/Acre,_Israel" ;
    foaf:topic "ACCO",
        "Management Accounting",
        "accounting",
        "decision making",
        "interdisciplinary",
        "qualitative" .

ex:ACCO435 a <http://www.dbpedia.org/resource/Course_(education)> ;
    rdfs:label "STRAT ACCTNG CASE ANALYSIS" ;
    focu:catalog "435" ;
    focu:credits 3.0 ;
    focu:offeredAt ex:Concordia ;
    focu:subject "ACCO" ;
    rdfs:comment "Please see UGRD Calendar" ;
    rdfs:seeAlso "('CASE', 'http://dbpedia.org/resource/Computer-aided_software_engineering')" ;
    foaf:topic "CASE" .

ex:ACCO440 a <http://www.dbpedia.org/resource/Course_(education)> ;
    rdfs:label "Advanced Taxation" ;
    focu:catalog "440" ;
    focu:credits 3.0 ;
    focu:offeredAt ex:Concordia ;
    focu:provenance "Concordia Open Data" ;
    focu:subject "ACCO" ;
    rdfs:comment """This course provides core knowledge regarding the federal taxation of corporations, partnerships, and trusts. It introduces analytical skills needed to make decisions regarding various business transfers, combinations, incorporation and estate planning issues for corporations and shareholders.
Prerequisite: ACCO 340.""" ;
    rdfs:seeAlso "http://dbpedia.org/resource/Acre,_Israel" ;
    foaf:topic "ACCO",
        "estate planning" .

ex:ACCO450 a <http://www.dbpedia.org/resource/Course_(education)> ;
    rdfs:label "Assurance Services" ;
    focu:catalog "450" ;
    focu:credits 3.0 ;
    focu:offeredAt ex:Concordia ;
    focu:provenance "Concordia Open Data" ;
    focu:subject "ACCO" ;
    rdfs:comment """This course examines the concepts and current standards of various assurance services, especially the audit of financial statements. It emphasizes the audit process and the role of the public accountant in expressing an opinion on the financial statements of an organization.
Prerequisite: ACCO 320 previously or concurrently.""" ;
    rdfs:seeAlso "http://dbpedia.org/resource/Acre,_Israel" ;
    foaf:topic "ACCO",
        "accountant",
        "assurance services",
        "audit",
        "financial statements" .

ex:ACCO455 a <http://www.dbpedia.org/resource/Course_(education)> ;
    rdfs:label "Fraud Prevention and Investigation" ;
    focu:catalog "455" ;
    focu:credits 3.0 ;
    focu:offeredAt ex:Concordia ;
    focu:provenance "Concordia Open Data" ;
    focu:subject "ACCO" ;
    rdfs:comment """This course examines the principles of and methodology used in fraud detection and deterrence. Topics covered may include skimming, cash larceny, cheque tampering, billing, payroll and expense reimbursement schemes, non-cash misappropriations, corruption, fraudulent financial statements, conducting investigations and interviewing witnesses. This course may also examine auditors' legal responsibilities towards fraud, the evaluation of internal controls and important pieces of legislation such as the Sarbanes-Oxley Act and the Criminal Code. Finally, the ethical aspects associated with fraud are discussed. Class sessions consist of lectures, real-life fraud case discussions and the presentation of DVDs from the Association of Certified Fraud Examiners.
Prerequisite: COMM 217, 315.
NOTE: Students who have received credit for this topic under an ACCO 470 number may not take this course for credit.""" ;
    rdfs:seeAlso "('Fraud', 'http://dbpedia.org/resource/Fraud')",
        "http://dbpedia.org/resource/Acre,_Israel" ;
    foaf:topic "ACCO",
        "Criminal Code",
        "Fraud",
        "Sarbanes-Oxley Act",
        "cheque",
        "corruption",
        "deterrence",
        "financial statements",
        "fraud",
        "fraud detection",
        "larceny",
        "skimming" .

ex:ACCO465 a <http://www.dbpedia.org/resource/Course_(education)> ;
    rdfs:label "Advanced Assurance Services" ;
    focu:catalog "465" ;
    focu:credits 3.0 ;
    focu:offeredAt ex:Concordia ;
    focu:provenance "Concordia Open Data" ;
    focu:subject "ACCO" ;
    rdfs:comment """This course covers important topics and concepts in auditing and assurance services. It builds on audit principles covered in previous courses and introduces specialized and advanced topics that are of particular importance to professional accountants. In covering topics and their application, the course focuses on decision-making processes followed by auditors. The course embraces the requirements of the CA Student Competency Map for assurance and the CGA Modules and Readings AU2.
Prerequisite: ACCO 320, 360; or ACCO 450.
NOTE: Students who have received credit for this topic under an ACCO 470 number may not take this course for credit.""" ;
    rdfs:seeAlso "http://dbpedia.org/resource/Acre,_Israel" ;
    foaf:topic "ACCO",
        "CA",
        "CGA",
        "assurance services",
        "audit",
        "auditing" .

ex:ACCO470 a <http://www.dbpedia.org/resource/Course_(education)> ;
    rdfs:label "SPECIAL TOPICS IN ACCOUNTING" ;
    focu:catalog "470" ;
    focu:credits 3.0 ;
    focu:offeredAt ex:Concordia ;
    focu:subject "ACCO" ;
    rdfs:comment "Please see UGRD Calendar" ;
    rdfs:seeAlso "('IN', 'http://dbpedia.org/resource/Indiana')" ;
    foaf:topic "IN" .

ex:ACCO471 a <http://www.dbpedia.org/resource/Course_(education)> ;
    rdfs:label "ACCOUNTING SEMINAR" ;
    focu:catalog "471" ;
    focu:credits 3.0 ;
    focu:offeredAt ex:Concordia ;
    focu:subject "ACCO" ;
    rdfs:comment "Please see UGRD Calendar" ;
    foaf:topic "No topics for this course" .

ex:ACCO590 a <http://www.dbpedia.org/resource/Course_(education)> ;
    rdfs:label "SPECIAL SEMINAR/ACCOUNTING" ;
    focu:catalog "590" ;
    focu:credits 1.0 ;
    focu:offeredAt ex:Concordia ;
    focu:subject "ACCO" ;
    rdfs:comment "Please see GRAD Calendar" ;
    foaf:topic "GRAD" .

ex:ACCO595 a <http://www.dbpedia.org/resource/Course_(education)> ;
    rdfs:label "SPECIAL TOPICS IN ACCO" ;
    focu:catalog "595" ;
    focu:credits 3.0 ;
    focu:offeredAt ex:Concordia ;
    focu:provenance "Concordia Open Data" ;
    focu:subject "ACCO" ;
    rdfs:comment "Please see GRAD Calendar" ;
    rdfs:seeAlso "('ACCO', 'http://dbpedia.org/resource/Acre,_Israel')",
        "http://dbpedia.org/resource/Acre,_Israel" ;
    foaf:topic "ACCO",
        "GRAD",
        "IN" .

ex:ACCO631 a <http://www.dbpedia.org/resource/Course_(education)> ;
    rdfs:label "BUSINESS ADVISORY SERVICES" ;
    focu:catalog "631" ;
    focu:credits 4.0 ;
    focu:offeredAt ex:Concordia ;
    focu:subject "ACCO" ;
    rdfs:comment "Please see GRAD Calendar" ;
    foaf:topic "GRAD" .

ex:ACCO631T a <http://www.dbpedia.org/resource/Course_(education)> ;
    rdfs:label "TUT/BSNSS ADVISORY SERVICES" ;
    focu:catalog "631T" ;
    focu:credits 4.0 ;
    focu:offeredAt ex:Concordia ;
    focu:subject "ACCO" ;
    rdfs:comment "Please see GRAD Calendar" ;
    rdfs:seeAlso "('TUT', 'http://dbpedia.org/resource/Tulip_Television')" ;
    foaf:topic "GRAD",
        "TUT" .

ex:ACCO635 a <http://www.dbpedia.org/resource/Course_(education)> ;
    rdfs:label "INTEGRATED APPROACH TO AUDIT" ;
    focu:catalog "635" ;
    focu:credits 4.0 ;
    focu:offeredAt ex:Concordia ;
    focu:subject "ACCO" ;
    rdfs:comment "Please see GRAD Calendar" ;
    foaf:topic "GRAD" .

ex:ACCO635T a <http://www.dbpedia.org/resource/Course_(education)> ;
    rdfs:label "TUT/INTEGRATED APPRO/AUDIT G" ;
    focu:catalog "635T" ;
    focu:credits 4.0 ;
    focu:offeredAt ex:Concordia ;
    focu:subject "ACCO" ;
    rdfs:comment "Please see GRAD Calendar" ;
    rdfs:seeAlso "('TUT', 'http://dbpedia.org/resource/Tulip_Television')" ;
    foaf:topic "GRAD",
        "TUT" .

ex:ACCO643X a <http://www.dbpedia.org/resource/Course_(education)> ;
    rdfs:label "SP TUTORIAL-INCOME TAXATION" ;
    focu:catalog "643X" ;
    focu:credits 1.0 ;
    focu:offeredAt ex:Concordia ;
    focu:subject "ACCO" ;
    rdfs:comment "Please see GRAD Calendar" ;
    rdfs:seeAlso "('SP', 'http://dbpedia.org/resource/Social_Democratic_Party_of_Switzerland')" ;
    foaf:topic "GRAD",
        "SP" .

ex:ACCO650 a <http://www.dbpedia.org/resource/Course_(education)> ;
    rdfs:label "FINA REPORTING IN PRACTICE" ;
    focu:catalog "650" ;
    focu:credits 4.0 ;
    focu:offeredAt ex:Concordia ;
    focu:subject "ACCO" ;
    rdfs:comment "Please see GRAD Calendar" ;
    rdfs:seeAlso "('FINA', 'http://dbpedia.org/resource/FINA')" ;
    foaf:topic "FINA",
        "GRAD",
        "IN" .

ex:ACCO650T a <http://www.dbpedia.org/resource/Course_(education)> ;
    rdfs:label "TUTORIAL IN FINA REP/PRACTICE" ;
    focu:catalog "650T" ;
    focu:credits 4.0 ;
    focu:offeredAt ex:Concordia ;
    focu:subject "ACCO" ;
    rdfs:comment "Please see GRAD Calendar" ;
    rdfs:seeAlso "('FINA', 'http://dbpedia.org/resource/FINA')" ;
    foaf:topic "FINA",
        "GRAD",
        "IN",
        "REP" .

ex:ACCO651 a <http://www.dbpedia.org/resource/Course_(education)> ;
    rdfs:label "FINANCIAL REPORTING:COMP APP" ;
    focu:catalog "651" ;
    focu:credits 4.0 ;
    focu:offeredAt ex:Concordia ;
    focu:subject "ACCO" ;
    rdfs:comment "Please see GRAD Calendar" ;
    rdfs:seeAlso "('APP', 'http://dbpedia.org/resource/Application_software')" ;
    foaf:topic "APP",
        "COMP",
        "GRAD" .

ex:ACCO651T a <http://www.dbpedia.org/resource/Course_(education)> ;
    rdfs:label "TUTORIAL IN FINA REP/COM APP" ;
    focu:catalog "651T" ;
    focu:credits 4.0 ;
    focu:offeredAt ex:Concordia ;
    focu:subject "ACCO" ;
    rdfs:comment "Please see GRAD Calendar" ;
    rdfs:seeAlso "('FINA', 'http://dbpedia.org/resource/FINA')" ;
    foaf:topic "APP",
        "FINA",
        "GRAD",
        "IN",
        "REP" .

ex:ACCO652 a <http://www.dbpedia.org/resource/Course_(education)> ;
    rdfs:label "BUSINESS ADVISORY SERVICES" ;
    focu:catalog "652" ;
    focu:credits 4.0 ;
    focu:offeredAt ex:Concordia ;
    focu:subject "ACCO" ;
    rdfs:comment "Please see GRAD Calendar" ;
    foaf:topic "GRAD" .

ex:ACCO652T a <http://www.dbpedia.org/resource/Course_(education)> ;
    rdfs:label "TUTORIAL IN BUSINESS ADV SER" ;
    focu:catalog "652T" ;
    focu:credits 4.0 ;
    focu:offeredAt ex:Concordia ;
    focu:subject "ACCO" ;
    rdfs:comment "Please see GRAD Calendar" ;
    rdfs:seeAlso "('SER', 'http://dbpedia.org/resource/Cadena_SER')" ;
    foaf:topic "ADV",
        "GRAD",
        "SER" .

ex:ACCO653 a <http://www.dbpedia.org/resource/Course_(education)> ;
    rdfs:label "INFO SYS/INTERNAL CONTROL" ;
    focu:catalog "653" ;
    focu:credits 4.0 ;
    focu:offeredAt ex:Concordia ;
    focu:subject "ACCO" ;
    rdfs:comment "Please see GRAD Calendar" ;
    rdfs:seeAlso "('SYS', 'http://dbpedia.org/resource/Sta._Elena_Construction_Wrecking_Balls')" ;
    foaf:topic "CONTROL",
        "GRAD",
        "SYS" .

ex:ACCO653T a <http://www.dbpedia.org/resource/Course_(education)> ;
    rdfs:label "TUTORIAL IN INF SYS/INT.CONT" ;
    focu:catalog "653T" ;
    focu:credits 4.0 ;
    focu:offeredAt ex:Concordia ;
    focu:subject "ACCO" ;
    rdfs:comment "Please see GRAD Calendar" ;
    rdfs:seeAlso "('SYS', 'http://dbpedia.org/resource/Sta._Elena_Construction_Wrecking_Balls')" ;
    foaf:topic "GRAD",
        "IN",
        "INF",
        "SYS" .

ex:ACCO655 a <http://www.dbpedia.org/resource/Course_(education)> ;
    rdfs:label "Taxation and Decision-Making" ;
    focu:catalog "655" ;
    focu:credits 4.0 ;
    focu:offeredAt ex:Concordia ;
    focu:subject "ACCO" ;
    rdfs:comment "Please see Graduate Calendar" ;
    foaf:topic "No topics for this course" .

ex:ACCO655T a <http://www.dbpedia.org/resource/Course_(education)> ;
    rdfs:label "Tutorial in Taxation/Decision making" ;
    focu:catalog "655T" ;
    focu:credits 4.0 ;
    focu:offeredAt ex:Concordia ;
    focu:subject "ACCO" ;
    rdfs:comment "Please see Graduate Calendar" ;
    rdfs:seeAlso "('Decision making', 'http://dbpedia.org/resource/Decision-making')" ;
    foaf:topic "Decision making" .

ex:ACCO658 a <http://www.dbpedia.org/resource/Course_(education)> ;
    rdfs:label "Capstone I Seminar" ;
    focu:catalog "658" ;
    focu:credits 2.0 ;
    focu:offeredAt ex:Concordia ;
    focu:subject "ACCO" ;
    rdfs:comment "Please see Graduate Calendar" ;
    foaf:topic "No topics for this course" .

ex:ACCO658T a <http://www.dbpedia.org/resource/Course_(education)> ;
    rdfs:label "Tutorial in Capstone I Seminar" ;
    focu:catalog "658T" ;
    focu:credits 2.0 ;
    focu:offeredAt ex:Concordia ;
    focu:subject "ACCO" ;
    rdfs:comment "Please see Graduate Calendar" ;
    foaf:topic "No topics for this course" .

ex:ACCO659 a <http://www.dbpedia.org/resource/Course_(education)> ;
    rdfs:label "Capstone II Examination Preparation" ;
    focu:catalog "659" ;
    focu:credits 4.0 ;
    focu:offeredAt ex:Concordia ;
    focu:subject "ACCO" ;
    rdfs:comment "Please see Graduate Calendar" ;
    rdfs:seeAlso "('II', 'http://dbpedia.org/resource/World_War_II')" ;
    foaf:topic "II" .

ex:ACCO672 a <http://www.dbpedia.org/resource/Course_(education)> ;
    rdfs:label "MANAGEMENT ACCOUNTING II" ;
    focu:catalog "672" ;
    focu:credits 3.0 ;
    focu:offeredAt ex:Concordia ;
    focu:subject "ACCO" ;
    rdfs:comment "Please see GRAD Calendar" ;
    rdfs:seeAlso "('II', 'http://dbpedia.org/resource/World_War_II')" ;
    foaf:topic "GRAD",
        "II" .

ex:ACCO681 a <http://www.dbpedia.org/resource/Course_(education)> ;
    rdfs:label "FINAN L ACCO G/REPORT G III" ;
    focu:catalog "681" ;
    focu:credits 3.0 ;
    focu:offeredAt ex:Concordia ;
    focu:provenance "Concordia Open Data" ;
    focu:subject "ACCO" ;
    rdfs:comment "Please see GRAD Calendar" ;
    rdfs:seeAlso "('III', 'http://dbpedia.org/resource/NCAA_Division_III')",
        "http://dbpedia.org/resource/Acre,_Israel" ;
    foaf:topic "ACCO",
        "FINAN",
        "GRAD" .

ex:ACCO682 a <http://www.dbpedia.org/resource/Course_(education)> ;
    rdfs:label "COMPREHENSIVE CASE ANALYSIS" ;
    focu:catalog "682" ;
    focu:credits 3.0 ;
    focu:offeredAt ex:Concordia ;
    focu:subject "ACCO" ;
    rdfs:comment "Please see GRAD Calendar" ;
    rdfs:seeAlso "('CASE', 'http://dbpedia.org/resource/Computer-aided_software_engineering')" ;
    foaf:topic "CASE",
        "GRAD" .

ex:ACCO685 a <http://www.dbpedia.org/resource/Course_(education)> ;
    rdfs:label "CASE ANALY/INTEG/EXAM PREP" ;
    focu:catalog "685" ;
    focu:credits 6.0 ;
    focu:offeredAt ex:Concordia ;
    focu:subject "ACCO" ;
    rdfs:comment "Please see GRAD Calendar" ;
    rdfs:seeAlso "('PREP', 'http://dbpedia.org/resource/PowerPC_Reference_Platform')" ;
    foaf:topic "CASE",
        "GRAD",
        "PREP" .

ex:ACCO690B a <http://www.dbpedia.org/resource/Course_(education)> ;
    rdfs:label "ADV EXAM WRITING TECHNIQUES" ;
    focu:catalog "690B" ;
    focu:credits 1.0 ;
    focu:offeredAt ex:Concordia ;
    focu:subject "ACCO" ;
    rdfs:comment "Please see GRAD Calendar" ;
    rdfs:seeAlso "('ADV', 'http://dbpedia.org/resource/A.D._Vision')" ;
    foaf:topic "ADV",
        "GRAD" .

ex:ACCO691 a <http://www.dbpedia.org/resource/Course_(education)> ;
    rdfs:label "SEMINAR-BUSINESS VALUATIONS" ;
    focu:catalog "691" ;
    focu:credits 3.0 ;
    focu:offeredAt ex:Concordia ;
    focu:subject "ACCO" ;
    rdfs:comment "Please see GRAD Calendar" ;
    foaf:topic "GRAD" .

ex:ACCO695 a <http://www.dbpedia.org/resource/Course_(education)> ;
    rdfs:label "SEMINAR IN SPECIAL TOPICS" ;
    focu:catalog "695" ;
    focu:credits 3.0 ;
    focu:offeredAt ex:Concordia ;
    focu:subject "ACCO" ;
    rdfs:comment "Please see GRAD Calendar" ;
    rdfs:seeAlso "('IN', 'http://dbpedia.org/resource/Indiana')" ;
    foaf:topic "GRAD" .

ex:ADV652T focu:provenance "Concordia Open Data" ;
    rdfs:seeAlso "http://dbpedia.org/resource/A.D._Vision" .

ex:ADV690B focu:provenance "Concordia Open Data" ;
    rdfs:seeAlso "http://dbpedia.org/resource/A.D._Vision" .

ex:AIS350 focu:provenance "Concordia Open Data" ;
    rdfs:seeAlso "http://dbpedia.org/resource/Association_for_Information_Systems" .

ex:APP651 focu:provenance "Concordia Open Data" ;
    rdfs:seeAlso "http://dbpedia.org/resource/Application_software" .

ex:APP651T focu:provenance "Concordia Open Data" ;
    rdfs:seeAlso "http://dbpedia.org/resource/Application_software" .

ex:Accounting230 focu:provenance "Concordia Open Data" ;
    rdfs:seeAlso "http://dbpedia.org/resource/Accounting" .

ex:Accounting350 focu:provenance "Concordia Open Data" ;
    rdfs:seeAlso "http://dbpedia.org/resource/Accounting" .

ex:Accounting400 focu:provenance "Concordia Open Data" ;
    rdfs:seeAlso "http://dbpedia.org/resource/Accounting" .

ex:CA465 focu:provenance "Concordia Open Data" ;
    rdfs:seeAlso "http://dbpedia.org/resource/Chartered_accountant" .

ex:CASE435 focu:provenance "Concordia Open Data" ;
    rdfs:seeAlso "http://dbpedia.org/resource/Computer-aided_software_engineering" .

ex:CASE682 focu:provenance "Concordia Open Data" ;
    rdfs:seeAlso "http://dbpedia.org/resource/Computer-aided_software_engineering" .

ex:CASE685 focu:provenance "Concordia Open Data" ;
    rdfs:seeAlso "http://dbpedia.org/resource/Computer-aided_software_engineering" .

ex:CGA465 focu:provenance "Concordia Open Data" ;
    rdfs:seeAlso "http://dbpedia.org/resource/Certified_General_Accountant" .

ex:COMP651 focu:provenance "Concordia Open Data" ;
    rdfs:seeAlso "http://dbpedia.org/resource/Cartilage_oligomeric_matrix_protein" .

ex:CONTROL653 focu:provenance "Concordia Open Data" ;
    rdfs:seeAlso "http://dbpedia.org/resource/Get_Smart" .

ex:Canada340 focu:provenance "Concordia Open Data" ;
    rdfs:seeAlso "http://dbpedia.org/resource/Canada" .

ex:Canadian340 focu:provenance "Concordia Open Data" ;
    rdfs:seeAlso "http://dbpedia.org/resource/Canada" .

ex:Criminal_Code455 focu:provenance "Concordia Open Data" ;
    rdfs:seeAlso "http://dbpedia.org/resource/Criminal_code" .

ex:Decision_making655T focu:provenance "Concordia Open Data" ;
    rdfs:seeAlso "http://dbpedia.org/resource/Decision-making" .

ex:FINA650 focu:provenance "Concordia Open Data" ;
    rdfs:seeAlso "http://dbpedia.org/resource/FINA" .

ex:FINA650T focu:provenance "Concordia Open Data" ;
    rdfs:seeAlso "http://dbpedia.org/resource/FINA" .

ex:FINA651T focu:provenance "Concordia Open Data" ;
    rdfs:seeAlso "http://dbpedia.org/resource/FINA" .

ex:FINAN681 focu:provenance "Concordia Open Data" ;
    rdfs:seeAlso "http://dbpedia.org/resource/Finan_of_Lindisfarne" .

ex:Fraud455 focu:provenance "Concordia Open Data" ;
    rdfs:seeAlso "http://dbpedia.org/resource/Fraud" .

ex:GRAD590 focu:provenance "Concordia Open Data" ;
    rdfs:seeAlso "http://dbpedia.org/resource/BM-21_Grad" .

ex:GRAD595 focu:provenance "Concordia Open Data" ;
    rdfs:seeAlso "http://dbpedia.org/resource/BM-21_Grad" .

ex:GRAD631 focu:provenance "Concordia Open Data" ;
    rdfs:seeAlso "http://dbpedia.org/resource/BM-21_Grad" .

ex:GRAD631T focu:provenance "Concordia Open Data" ;
    rdfs:seeAlso "http://dbpedia.org/resource/BM-21_Grad" .

ex:GRAD635 focu:provenance "Concordia Open Data" ;
    rdfs:seeAlso "http://dbpedia.org/resource/BM-21_Grad" .

ex:GRAD635T focu:provenance "Concordia Open Data" ;
    rdfs:seeAlso "http://dbpedia.org/resource/BM-21_Grad" .

ex:GRAD643X focu:provenance "Concordia Open Data" ;
    rdfs:seeAlso "http://dbpedia.org/resource/BM-21_Grad" .

ex:GRAD650 focu:provenance "Concordia Open Data" ;
    rdfs:seeAlso "http://dbpedia.org/resource/BM-21_Grad" .

ex:GRAD650T focu:provenance "Concordia Open Data" ;
    rdfs:seeAlso "http://dbpedia.org/resource/BM-21_Grad" .

ex:GRAD651 focu:provenance "Concordia Open Data" ;
    rdfs:seeAlso "http://dbpedia.org/resource/BM-21_Grad" .

ex:GRAD651T focu:provenance "Concordia Open Data" ;
    rdfs:seeAlso "http://dbpedia.org/resource/BM-21_Grad" .

ex:GRAD652 focu:provenance "Concordia Open Data" ;
    rdfs:seeAlso "http://dbpedia.org/resource/BM-21_Grad" .

ex:GRAD652T focu:provenance "Concordia Open Data" ;
    rdfs:seeAlso "http://dbpedia.org/resource/BM-21_Grad" .

ex:GRAD653 focu:provenance "Concordia Open Data" ;
    rdfs:seeAlso "http://dbpedia.org/resource/BM-21_Grad" .

ex:GRAD653T focu:provenance "Concordia Open Data" ;
    rdfs:seeAlso "http://dbpedia.org/resource/BM-21_Grad" .

ex:GRAD672 focu:provenance "Concordia Open Data" ;
    rdfs:seeAlso "http://dbpedia.org/resource/BM-21_Grad" .

ex:GRAD681 focu:provenance "Concordia Open Data" ;
    rdfs:seeAlso "http://dbpedia.org/resource/BM-21_Grad" .

ex:GRAD682 focu:provenance "Concordia Open Data" ;
    rdfs:seeAlso "http://dbpedia.org/resource/BM-21_Grad" .

ex:GRAD685 focu:provenance "Concordia Open Data" ;
    rdfs:seeAlso "http://dbpedia.org/resource/BM-21_Grad" .

ex:GRAD690B focu:provenance "Concordia Open Data" ;
    rdfs:seeAlso "http://dbpedia.org/resource/BM-21_Grad" .

ex:GRAD691 focu:provenance "Concordia Open Data" ;
    rdfs:seeAlso "http://dbpedia.org/resource/BM-21_Grad" .

ex:GRAD695 focu:provenance "Concordia Open Data" ;
    rdfs:seeAlso "http://dbpedia.org/resource/BM-21_Grad" .

ex:II320 focu:provenance "Concordia Open Data" ;
    rdfs:seeAlso "http://dbpedia.org/resource/World_War_II" .

ex:II659 focu:provenance "Concordia Open Data" ;
    rdfs:seeAlso "http://dbpedia.org/resource/World_War_II" .

ex:II672 focu:provenance "Concordia Open Data" ;
    rdfs:seeAlso "http://dbpedia.org/resource/World_War_II" .

ex:IN470 focu:provenance "Concordia Open Data" ;
    rdfs:seeAlso "http://dbpedia.org/resource/Indiana" .

ex:IN595 focu:provenance "Concordia Open Data" ;
    rdfs:seeAlso "http://dbpedia.org/resource/Indiana" .

ex:IN650 focu:provenance "Concordia Open Data" ;
    rdfs:seeAlso "http://dbpedia.org/resource/Indiana" .

ex:IN650T focu:provenance "Concordia Open Data" ;
    rdfs:seeAlso "http://dbpedia.org/resource/Indiana" .

ex:IN651T focu:provenance "Concordia Open Data" ;
    rdfs:seeAlso "http://dbpedia.org/resource/Indiana" .

ex:IN653T focu:provenance "Concordia Open Data" ;
    rdfs:seeAlso "http://dbpedia.org/resource/Indiana" .

ex:INF653T focu:provenance "Concordia Open Data" ;
    rdfs:seeAlso "http://dbpedia.org/resource/INF_file" .

ex:IV425 focu:provenance "Concordia Open Data" ;
    rdfs:seeAlso "http://dbpedia.org/resource/Intravenous_therapy" .

ex:Information_Technology350 focu:provenance "Concordia Open Data" ;
    rdfs:seeAlso "http://dbpedia.org/resource/Information_technology" .

ex:Management_Accounting330 focu:provenance "Concordia Open Data" ;
    rdfs:seeAlso "http://dbpedia.org/resource/Management_accounting" .

ex:Management_Accounting430 focu:provenance "Concordia Open Data" ;
    rdfs:seeAlso "http://dbpedia.org/resource/Management_accounting" .

ex:Managerial_Accounting220 focu:provenance "Concordia Open Data" ;
    rdfs:seeAlso "http://dbpedia.org/resource/Management_accounting" .

ex:Managerial_Accounting240 focu:provenance "Concordia Open Data" ;
    rdfs:seeAlso "http://dbpedia.org/resource/Management_accounting" .

ex:PREP685 focu:provenance "Concordia Open Data" ;
    rdfs:seeAlso "http://dbpedia.org/resource/PowerPC_Reference_Platform" .

ex:REP650T focu:provenance "Concordia Open Data" ;
    rdfs:seeAlso "http://dbpedia.org/resource/Robert_Esnault-Pelterie" .

ex:REP651T focu:provenance "Concordia Open Data" ;
    rdfs:seeAlso "http://dbpedia.org/resource/Robert_Esnault-Pelterie" .

ex:SER652T focu:provenance "Concordia Open Data" ;
    rdfs:seeAlso "http://dbpedia.org/resource/Cadena_SER" .

ex:SP643X focu:provenance "Concordia Open Data" ;
    rdfs:seeAlso "http://dbpedia.org/resource/Social_Democratic_Party_of_Switzerland" .

ex:SYS653 focu:provenance "Concordia Open Data" ;
    rdfs:seeAlso "http://dbpedia.org/resource/Sta._Elena_Construction_Wrecking_Balls" .

ex:SYS653T focu:provenance "Concordia Open Data" ;
    rdfs:seeAlso "http://dbpedia.org/resource/Sta._Elena_Construction_Wrecking_Balls" .

ex:Sarbanes-Oxley_Act455 focu:provenance "Concordia Open Data" ;
    rdfs:seeAlso "http://dbpedia.org/resource/Sarbanes–Oxley_Act" .

ex:TUT631T focu:provenance "Concordia Open Data" ;
    rdfs:seeAlso "http://dbpedia.org/resource/Tulip_Television" .

ex:TUT635T focu:provenance "Concordia Open Data" ;
    rdfs:seeAlso "http://dbpedia.org/resource/Tulip_Television" .

ex:U.S.365 focu:provenance "Concordia Open Data" ;
    rdfs:seeAlso "http://dbpedia.org/resource/United_States" .

ex:accountant450 focu:provenance "Concordia Open Data" ;
    rdfs:seeAlso "http://dbpedia.org/resource/Management_accounting" .

ex:accounting220 focu:provenance "Concordia Open Data" ;
    rdfs:seeAlso "http://dbpedia.org/resource/Accounting" .

ex:accounting230 focu:provenance "Concordia Open Data" ;
    rdfs:seeAlso "http://dbpedia.org/resource/Accounting" .

ex:accounting240 focu:provenance "Concordia Open Data" ;
    rdfs:seeAlso "http://dbpedia.org/resource/Accounting" .

ex:accounting320 focu:provenance "Concordia Open Data" ;
    rdfs:seeAlso "http://dbpedia.org/resource/Accounting" .

ex:accounting330 focu:provenance "Concordia Open Data" ;
    rdfs:seeAlso "http://dbpedia.org/resource/Accounting" .

ex:accounting350 focu:provenance "Concordia Open Data" ;
    rdfs:seeAlso "http://dbpedia.org/resource/Accounting" .

ex:accounting400 focu:provenance "Concordia Open Data" ;
    rdfs:seeAlso "http://dbpedia.org/resource/Accounting" .

ex:accounting420 focu:provenance "Concordia Open Data" ;
    rdfs:seeAlso "http://dbpedia.org/resource/Accounting" .

ex:accounting430 focu:provenance "Concordia Open Data" ;
    rdfs:seeAlso "http://dbpedia.org/resource/Accounting" .

ex:assurance_services450 focu:provenance "Concordia Open Data" ;
    rdfs:seeAlso "http://dbpedia.org/resource/Assurance_services" .

ex:assurance_services465 focu:provenance "Concordia Open Data" ;
    rdfs:seeAlso "http://dbpedia.org/resource/Assurance_services" .

ex:audit450 focu:provenance "Concordia Open Data" ;
    rdfs:seeAlso "http://dbpedia.org/resource/Audit" .

ex:audit465 focu:provenance "Concordia Open Data" ;
    rdfs:seeAlso "http://dbpedia.org/resource/Audit" .

ex:auditing465 focu:provenance "Concordia Open Data" ;
    rdfs:seeAlso "http://dbpedia.org/resource/Audit" .

ex:capital_gains340 focu:provenance "Concordia Open Data" ;
    rdfs:seeAlso "http://dbpedia.org/resource/Capital_gain" .

ex:cheque455 focu:provenance "Concordia Open Data" ;
    rdfs:seeAlso "http://dbpedia.org/resource/Cheque" .

ex:computer350 focu:provenance "Concordia Open Data" ;
    rdfs:seeAlso "http://dbpedia.org/resource/Computer" .

ex:conceptual_framework400 focu:provenance "Concordia Open Data" ;
    rdfs:seeAlso "http://dbpedia.org/resource/Conceptual_framework" .

ex:corporate_taxation365 focu:provenance "Concordia Open Data" ;
    rdfs:seeAlso "http://dbpedia.org/resource/Corporate_tax" .

ex:corruption455 focu:provenance "Concordia Open Data" ;
    rdfs:seeAlso "http://dbpedia.org/resource/Political_corruption" .

ex:currency420 focu:provenance "Concordia Open Data" ;
    rdfs:seeAlso "http://dbpedia.org/resource/Currency" .

ex:decision_making240 focu:provenance "Concordia Open Data" ;
    rdfs:seeAlso "http://dbpedia.org/resource/Decision-making" .

ex:decision_making350 focu:provenance "Concordia Open Data" ;
    rdfs:seeAlso "http://dbpedia.org/resource/Decision-making" .

ex:decision_making430 focu:provenance "Concordia Open Data" ;
    rdfs:seeAlso "http://dbpedia.org/resource/Decision-making" .

ex:deterrence455 focu:provenance "Concordia Open Data" ;
    rdfs:seeAlso "http://dbpedia.org/resource/Deterrence_theory" .

ex:e-business350 focu:provenance "Concordia Open Data" ;
    rdfs:seeAlso "http://dbpedia.org/resource/Electronic_business" .

ex:estate_planning440 focu:provenance "Concordia Open Data" ;
    rdfs:seeAlso "http://dbpedia.org/resource/Estate_planning" .

ex:federal_income_tax340 focu:provenance "Concordia Open Data" ;
    rdfs:seeAlso "http://dbpedia.org/resource/Income_tax_in_the_United_States" .

ex:financial_reporting310 focu:provenance "Concordia Open Data" ;
    rdfs:seeAlso "http://dbpedia.org/resource/Financial_statement" .

ex:financial_reporting400 focu:provenance "Concordia Open Data" ;
    rdfs:seeAlso "http://dbpedia.org/resource/Financial_statement" .

ex:financial_statement_analysis355 focu:provenance "Concordia Open Data" ;
    rdfs:seeAlso "http://dbpedia.org/resource/Financial_statement_analysis" .

ex:financial_statements230 focu:provenance "Concordia Open Data" ;
    rdfs:seeAlso "http://dbpedia.org/resource/Financial_statement" .

ex:financial_statements355 focu:provenance "Concordia Open Data" ;
    rdfs:seeAlso "http://dbpedia.org/resource/Financial_statement" .

ex:financial_statements420 focu:provenance "Concordia Open Data" ;
    rdfs:seeAlso "http://dbpedia.org/resource/Financial_statement" .

ex:financial_statements450 focu:provenance "Concordia Open Data" ;
    rdfs:seeAlso "http://dbpedia.org/resource/Financial_statement" .

ex:financial_statements455 focu:provenance "Concordia Open Data" ;
    rdfs:seeAlso "http://dbpedia.org/resource/Financial_statement" .

ex:fraud350 focu:provenance "Concordia Open Data" ;
    rdfs:seeAlso "http://dbpedia.org/resource/Fraud" .

ex:fraud455 focu:provenance "Concordia Open Data" ;
    rdfs:seeAlso "http://dbpedia.org/resource/Fraud" .

ex:fraud_detection455 focu:provenance "Concordia Open Data" ;
    rdfs:seeAlso "http://dbpedia.org/resource/Fraud" .

ex:goods340 focu:provenance "Concordia Open Data" ;
    rdfs:seeAlso "http://dbpedia.org/resource/Goods" .

ex:interdisciplinary430 focu:provenance "Concordia Open Data" ;
    rdfs:seeAlso "http://dbpedia.org/resource/Interdisciplinarity" .

ex:larceny455 focu:provenance "Concordia Open Data" ;
    rdfs:seeAlso "http://dbpedia.org/resource/Larceny" .

ex:liabilities320 focu:provenance "Concordia Open Data" ;
    rdfs:seeAlso "http://dbpedia.org/resource/Asset" .

ex:pension320 focu:provenance "Concordia Open Data" ;
    rdfs:seeAlso "http://dbpedia.org/resource/Pension" .

ex:process_costing330 focu:provenance "Concordia Open Data" ;
    rdfs:seeAlso "http://dbpedia.org/resource/Process_costing" .

ex:property_income340 focu:provenance "Concordia Open Data" ;
    rdfs:seeAlso "http://dbpedia.org/resource/Property_income" .

ex:qualitative430 focu:provenance "Concordia Open Data" ;
    rdfs:seeAlso "http://dbpedia.org/resource/Qualitative_research" .

<http://example.org/shareholders'_equity320> focu:provenance "Concordia Open Data" ;
    rdfs:seeAlso "http://dbpedia.org/resource/Equity_(finance)" .

ex:skimming455 focu:provenance "Concordia Open Data" ;
    rdfs:seeAlso "http://dbpedia.org/resource/Credit_card_fraud" .

ex:systems_analysis350 focu:provenance "Concordia Open Data" ;
    rdfs:seeAlso "http://dbpedia.org/resource/Systems_analysis" .

ex:tax340 focu:provenance "Concordia Open Data" ;
    rdfs:seeAlso "http://dbpedia.org/resource/Tax" .

ex:tax_planning365 focu:provenance "Concordia Open Data" ;
    rdfs:seeAlso "http://dbpedia.org/resource/Tax_avoidance" .

ex:transfer_pricing330 focu:provenance "Concordia Open Data" ;
    rdfs:seeAlso "http://dbpedia.org/resource/Transfer_pricing" .

ex:variance_analysis330 focu:provenance "Concordia Open Data" ;
    rdfs:seeAlso "http://dbpedia.org/resource/Analysis_of_variance" .

focu:Record a dbo:document ;
    rdfs:label "Record"@en ;
    rdfs:comment "Information about single student's participation in a single course in a particular semester"@en .

focu:catalog a rdf:Property ;
    rdfs:label "Course number"@en ;
    rdfs:comment "An integer number which uniquely identifies a course within a particular discipline."@en ;
    rdfs:domain <http://www.dbpedia.org/resource/Course_(education)> ;
    rdfs:range xsd:string .

focu:course a rdf:Property ;
    rdfs:label "Unique identifier for a course"@en ;
    rdfs:comment "An abbreviated course displicine and course number which combined uniquely identifies any university course within that academic institution."@en ;
    rdfs:domain ex:Record ;
    rdfs:range xsd:string .

focu:credits a rdf:Property ;
    rdfs:label "Letter grade"@en ;
    rdfs:comment "A single letter measuring the performance in the course of the associated Record."@en ;
    rdfs:domain <http://www.dbpedia.org/resource/Course_(education)> ;
    rdfs:range xsd:int .

focu:grade a rdf:Property ;
    rdfs:label "Letter grade"@en ;
    rdfs:comment "A single letter measuring the performance in the course of the associated Record."@en ;
    rdfs:domain ex:Record ;
    rdfs:range xsd:string .

focu:hasRecord a rdf:Property ;
    rdfs:label "Has record"@en ;
    rdfs:comment "A property describing the relationship between a single student and a single record"@en ;
    rdfs:domain ex:Student ;
    rdfs:range ex:Record .

focu:offeredAt a rdf:Property ;
    rdfs:label "Offered At"@en ;
    rdfs:comment "A university course is offered at the associated university."@en ;
    rdfs:domain <http://www.dbpedia.org/resource/Course_(education)> ;
    rdfs:range dbr:Public_university .

focu:provenance a rdf:Property ;
    rdfs:label "Provenance"@en ;
    rdfs:comment "Record of where the topic was identified as being covered in the course"@en ;
    rdfs:domain foaf:topic ;
    rdfs:range xsd:string .

focu:semester a rdf:Property ;
    rdfs:label "Semester"@en ;
    rdfs:comment "The year in which the course associated to the Record took place."@en ;
    rdfs:domain ex:Record ;
    rdfs:range xsd:string .

focu:subject a rdf:Property ;
    rdfs:label "Discipline of course"@en ;
    rdfs:comment "An abbreviation for the discipline or department under which an academic course falls"@en ;
    rdfs:domain <http://www.dbpedia.org/resource/Course_(education)> ;
    rdfs:range xsd:string .

ex:Concordia dbo:type dbr:Public_university ;
    rdfs:seeAlso dbr:Concordia_University ;
    foaf:name "Concordia University" .

